proofs/isabelle/SpecRest/SchemaDiff.thy
@@ -11,120 +11,120 @@ text \<open>Pure schema-diff: given two schemas plus their dialect-rewritten nam
 type_synonym check_pair    = "String.literal \<times> String.literal"
 type_synonym check_assign  = "(String.literal \<times> check_pair list) list"
 
-definition lookup_checks :: "String.literal \<Rightarrow> check_assign \<Rightarrow> check_pair list"
+definition lookupChecks :: "String.literal \<Rightarrow> check_assign \<Rightarrow> check_pair list"
 where
-  "lookup_checks tn assigns = (case map_of assigns tn of None \<Rightarrow> [] | Some cs \<Rightarrow> cs)"
+  "lookupChecks tn assigns = (case map_of assigns tn of None \<Rightarrow> [] | Some cs \<Rightarrow> cs)"
 
-definition column_names :: "table_spec \<Rightarrow> String.literal list"
+definition columnNames :: "table_spec \<Rightarrow> String.literal list"
 where
-  "column_names t = map column_name (table_columns t)"
+  "columnNames t = map columnName (tableColumns t)"
 
-definition intra_drops ::
+definition intraDrops ::
   "table_spec \<Rightarrow> table_spec \<Rightarrow> check_pair list \<Rightarrow> check_pair list \<Rightarrow> migration_op list"
 where
-  "intra_drops prev nxt prev_cks nxt_cks \<equiv>
-    let tn = table_name prev;
-        nxt_col_set = set (column_names nxt);
+  "intraDrops prev nxt prev_cks nxt_cks \<equiv>
+    let tn = tableName prev;
+        nxt_col_set = set (columnNames nxt);
         drop_col_ops = map (\<lambda>c. DropColumn tn c)
-                         (filter (\<lambda>c. column_name c \<notin> nxt_col_set) (table_columns prev));
-        nxt_ix_set = set (table_indexes nxt);
+                         (filter (\<lambda>c. columnName c \<notin> nxt_col_set) (tableColumns prev));
+        nxt_ix_set = set (tableIndexes nxt);
         drop_ix_ops = map (\<lambda>i. DropIndex tn i)
-                        (filter (\<lambda>i. i \<notin> nxt_ix_set) (table_indexes prev));
-        nxt_fk_set = set (table_foreign_keys nxt);
+                        (filter (\<lambda>i. i \<notin> nxt_ix_set) (tableIndexes prev));
+        nxt_fk_set = set (tableForeignKeys nxt);
         drop_fk_ops = map (\<lambda>f. DropForeignKey tn f)
-                        (filter (\<lambda>f. f \<notin> nxt_fk_set) (table_foreign_keys prev));
+                        (filter (\<lambda>f. f \<notin> nxt_fk_set) (tableForeignKeys prev));
         nxt_ck_set = set nxt_cks;
         drop_ck_ops = map (\<lambda>p. DropCheck tn (fst p) (snd p))
                         (filter (\<lambda>p. p \<notin> nxt_ck_set) prev_cks)
     in drop_ix_ops @ drop_ck_ops @ drop_fk_ops @ drop_col_ops"
 
-definition intra_adds ::
+definition intraAdds ::
   "table_spec \<Rightarrow> table_spec \<Rightarrow> check_pair list \<Rightarrow> check_pair list \<Rightarrow> migration_op list"
 where
-  "intra_adds prev nxt prev_cks nxt_cks \<equiv>
-    let tn = table_name nxt;
-        prev_col_set = set (column_names prev);
+  "intraAdds prev nxt prev_cks nxt_cks \<equiv>
+    let tn = tableName nxt;
+        prev_col_set = set (columnNames prev);
         add_col_ops = map (\<lambda>c. AddColumn tn c)
-                        (filter (\<lambda>c. column_name c \<notin> prev_col_set) (table_columns nxt));
-        prev_ix_set = set (table_indexes prev);
+                        (filter (\<lambda>c. columnName c \<notin> prev_col_set) (tableColumns nxt));
+        prev_ix_set = set (tableIndexes prev);
         add_ix_ops = map (\<lambda>i. AddIndex tn i)
-                       (filter (\<lambda>i. i \<notin> prev_ix_set) (table_indexes nxt));
-        prev_fk_set = set (table_foreign_keys prev);
+                       (filter (\<lambda>i. i \<notin> prev_ix_set) (tableIndexes nxt));
+        prev_fk_set = set (tableForeignKeys prev);
         add_fk_ops = map (\<lambda>f. AddForeignKey tn f)
-                       (filter (\<lambda>f. f \<notin> prev_fk_set) (table_foreign_keys nxt));
+                       (filter (\<lambda>f. f \<notin> prev_fk_set) (tableForeignKeys nxt));
         prev_ck_set = set prev_cks;
         add_ck_ops = map (\<lambda>p. AddCheck tn (fst p) (snd p))
                        (filter (\<lambda>p. p \<notin> prev_ck_set) nxt_cks)
     in add_col_ops @ add_fk_ops @ add_ck_ops @ add_ix_ops"
 
-definition alter_for_pair :: "String.literal \<Rightarrow> column_spec \<Rightarrow> column_spec \<Rightarrow> migration_op list"
+definition alterForPair :: "String.literal \<Rightarrow> column_spec \<Rightarrow> column_spec \<Rightarrow> migration_op list"
 where
-  "alter_for_pair tn pc nc \<equiv>
+  "alterForPair tn pc nc \<equiv>
     let type_change =
-          (if column_sql_type pc = column_sql_type nc then []
-           else [AlterColumnType tn (column_name nc) (column_sql_type pc) (column_sql_type nc)]);
+          (if columnSqlType pc = columnSqlType nc then []
+           else [AlterColumnType tn (columnName nc) (columnSqlType pc) (columnSqlType nc)]);
         null_change =
-          (if column_nullable pc = column_nullable nc then []
-           else [AlterColumnNullable tn (column_name nc) (column_nullable pc) (column_nullable nc)]);
+          (if columnNullable pc = columnNullable nc then []
+           else [AlterColumnNullable tn (columnName nc) (columnNullable pc) (columnNullable nc)]);
         def_change =
-          (if column_default_value pc = column_default_value nc then []
-           else [AlterColumnDefault tn (column_name nc) (column_default_value pc) (column_default_value nc)])
+          (if columnDefaultValue pc = columnDefaultValue nc then []
+           else [AlterColumnDefault tn (columnName nc) (columnDefaultValue pc) (columnDefaultValue nc)])
     in type_change @ null_change @ def_change"
 
-definition intra_alters :: "table_spec \<Rightarrow> table_spec \<Rightarrow> migration_op list"
+definition intraAlters :: "table_spec \<Rightarrow> table_spec \<Rightarrow> migration_op list"
 where
-  "intra_alters prev nxt \<equiv>
-    let prev_cols = map (\<lambda>c. (column_name c, c)) (table_columns prev)
+  "intraAlters prev nxt \<equiv>
+    let prev_cols = map (\<lambda>c. (columnName c, c)) (tableColumns prev)
     in concat (map (\<lambda>nc.
-        case map_of prev_cols (column_name nc) of
+        case map_of prev_cols (columnName nc) of
           None \<Rightarrow> []
-        | Some pc \<Rightarrow> alter_for_pair (table_name nxt) pc nc
-       ) (table_columns nxt))"
+        | Some pc \<Rightarrow> alterForPair (tableName nxt) pc nc
+       ) (tableColumns nxt))"
 
 text \<open>Topo-sort the given tables, then map names back to their table_spec.
   Returns the input order on cycle (matches the Scala fallback when extracted topo_sort
   returns None — caller validates).\<close>
 
-definition sort_tables_by_fk :: "table_spec list \<Rightarrow> table_spec list option"
+definition sortTablesByFk :: "table_spec list \<Rightarrow> table_spec list option"
 where
-  "sort_tables_by_fk ts \<equiv>
-    (case topo_sort_names (table_dep_pairs ts) of
+  "sortTablesByFk ts \<equiv>
+    (case topoSortNames (tableDepPairs ts) of
        None \<Rightarrow> None
      | Some ns \<Rightarrow>
-         let by_name = map (\<lambda>t. (table_name t, t)) ts in
+         let by_name = map (\<lambda>t. (tableName t, t)) ts in
          Some (concat (map (\<lambda>n. case map_of by_name n of None \<Rightarrow> [] | Some t \<Rightarrow> [t]) ns)))"
 
-definition compute_diff ::
+definition computeDiff ::
   "database_schema \<Rightarrow> database_schema \<Rightarrow> check_assign \<Rightarrow> check_assign
    \<Rightarrow> migration_op list option"
 where
-  "compute_diff prev nxt prev_cks nxt_cks \<equiv>
-    let prev_ts = schema_tables prev;
-        nxt_ts  = schema_tables nxt;
-        prev_names = map table_name prev_ts;
-        nxt_names  = map table_name nxt_ts;
-        prev_by_name = map (\<lambda>t. (table_name t, t)) prev_ts;
+  "computeDiff prev nxt prev_cks nxt_cks \<equiv>
+    let prev_ts = schemaTables prev;
+        nxt_ts  = schemaTables nxt;
+        prev_names = map tableName prev_ts;
+        nxt_names  = map tableName nxt_ts;
+        prev_by_name = map (\<lambda>t. (tableName t, t)) prev_ts;
         kept_pairs = concat (map (\<lambda>n.
-                       case map_of prev_by_name (table_name n) of
+                       case map_of prev_by_name (tableName n) of
                          None \<Rightarrow> []
                        | Some p \<Rightarrow> [(p, n)]) nxt_ts);
         drops_inside = concat (map (\<lambda>pn.
-                         intra_drops (fst pn) (snd pn)
-                           (lookup_checks (table_name (snd pn)) prev_cks)
-                           (lookup_checks (table_name (snd pn)) nxt_cks)) kept_pairs);
+                         intraDrops (fst pn) (snd pn)
+                           (lookupChecks (tableName (snd pn)) prev_cks)
+                           (lookupChecks (tableName (snd pn)) nxt_cks)) kept_pairs);
         adds_inside  = concat (map (\<lambda>pn.
-                         intra_adds (fst pn) (snd pn)
-                           (lookup_checks (table_name (snd pn)) prev_cks)
-                           (lookup_checks (table_name (snd pn)) nxt_cks)) kept_pairs);
-        alters_inside = concat (map (\<lambda>pn. intra_alters (fst pn) (snd pn)) kept_pairs);
-        dropped_table_specs = filter (\<lambda>t. table_name t \<notin> set nxt_names) prev_ts;
-        created_table_specs = filter (\<lambda>t. table_name t \<notin> set prev_names) nxt_ts;
-        prev_trg = schema_triggers prev;
-        nxt_trg  = schema_triggers nxt;
+                         intraAdds (fst pn) (snd pn)
+                           (lookupChecks (tableName (snd pn)) prev_cks)
+                           (lookupChecks (tableName (snd pn)) nxt_cks)) kept_pairs);
+        alters_inside = concat (map (\<lambda>pn. intraAlters (fst pn) (snd pn)) kept_pairs);
+        dropped_table_specs = filter (\<lambda>t. tableName t \<notin> set nxt_names) prev_ts;
+        created_table_specs = filter (\<lambda>t. tableName t \<notin> set prev_names) nxt_ts;
+        prev_trg = schemaTriggers prev;
+        nxt_trg  = schemaTriggers nxt;
         dropped_triggers = map DropTrigger (filter (\<lambda>t. t \<notin> set nxt_trg) prev_trg);
         added_triggers   = map AddTrigger  (filter (\<lambda>t. t \<notin> set prev_trg) nxt_trg)
     in
-      case (sort_tables_by_fk dropped_table_specs, sort_tables_by_fk created_table_specs) of
+      case (sortTablesByFk dropped_table_specs, sortTablesByFk created_table_specs) of
         (Some dts, Some cts) \<Rightarrow>
           Some (dropped_triggers
                 @ drops_inside
@@ -135,13 +135,13 @@ where
                 @ added_triggers)
       | _ \<Rightarrow> None"
 
-lemmas compute_diff_code [code] = compute_diff_def
-lemmas intra_drops_code [code]  = intra_drops_def
-lemmas intra_adds_code [code]   = intra_adds_def
-lemmas intra_alters_code [code] = intra_alters_def
-lemmas alter_for_pair_code [code] = alter_for_pair_def
-lemmas sort_tables_by_fk_code [code] = sort_tables_by_fk_def
-lemmas lookup_checks_code [code] = lookup_checks_def
-lemmas column_names_code [code] = column_names_def
+lemmas computeDiffCode [code] = computeDiff_def
+lemmas intraDropsCode [code]  = intraDrops_def
+lemmas intraAddsCode [code]   = intraAdds_def
+lemmas intraAltersCode [code] = intraAlters_def
+lemmas alterForPairCode [code] = alterForPair_def
+lemmas sortTablesByFkCode [code] = sortTablesByFk_def
+lemmas lookupChecksCode [code] = lookupChecks_def
+lemmas columnNamesCode [code] = columnNames_def
 
 end
